compiler/src/Common/Data/DatatoEJSON.v
@@ -1,0 +1,349 @@
+(*
+ * Copyright 2015-2016 IBM Corporation
+ *
+ * Licensed under the Apache License, Version 2.0 (the "License");
+ * you may not use this file except in compliance with the License.
+ * You may obtain a copy of the License at
+ *
+ * http://www.apache.org/licenses/LICENSE-2.0
+ *
+ * Unless required by applicable law or agreed to in writing, software
+ * distributed under the License is distributed on an "AS IS" BASIS,
+ * WITHOUT WARRANTIES OR CONDITIONS OF ANY KIND, either express or implied.
+ * See the License for the specific language governing permissions and
+ * limitations under the License.
+ *)
+
+Require Import List.
+Require Import String.
+Require Import Ascii.
+Require Import ZArith.
+Require Import Utils.
+Require Import ForeignEJSON.
+Require Import EJSON.
+Require Import ForeignData.
+Require Import ForeignDataToEJSON.
+Require Import Data.
+Require Import DataNorm.
+
+Section DatatoEJSON.
+  Context {fdata:foreign_data}.
+  Context {ftoejson:foreign_ejson}.
+  Context {fdatatoejson:foreign_to_ejson}.
+
+  Section toData.
+    (* EJSON to Data *)
+
+    Fixpoint ejson_brands (d:list ejson) : option (list string) :=
+      match d with
+      | nil => Some nil
+      | (ejstring s1) :: d' =>
+        match ejson_brands d' with
+        | Some s' => Some (s1::s')
+        | None => None
+        end
+      | _ => None
+      end.
+
+    Fixpoint ejson_to_data_pre (j:ejson) : data :=
+      match j with
+      | ejnull => dunit
+      | ejnumber n => dfloat n
+      | ejbigint n => dnat n
+      | ejbool b => dbool b
+      | ejstring s => dstring s
+      | ejarray c => dcoll (map ejson_to_data_pre c)
+      | ejobject nil => drec nil
+      | ejobject ((s1,j')::nil) =>
+        if (string_dec s1 "$left") then dleft (ejson_to_data_pre j')
+        else if (string_dec s1 "$right") then dright (ejson_to_data_pre j')
+             else drec ((json_key_decode s1, ejson_to_data_pre j')::nil)
+      | ejobject ((s1,ejarray j1)::(s2,j2)::nil) =>
+        if (string_dec s1 "$type") then
+          if (string_dec s2 "$data") then
+            match (ejson_brands j1) with
+            | Some br => dbrand br (ejson_to_data_pre j2)
+            | None => drec ((json_key_decode s1, dcoll (map ejson_to_data_pre j1))::(json_key_decode s2, ejson_to_data_pre j2)::nil)
+            end
+          else drec ((json_key_decode s1, dcoll (map ejson_to_data_pre j1))::(json_key_decode s2, ejson_to_data_pre j2)::nil)
+        else drec ((json_key_decode s1, dcoll (map ejson_to_data_pre j1))::(json_key_decode s2, ejson_to_data_pre j2)::nil)
+      | ejobject ((s1,j1)::(s2,ejarray j2)::nil) =>
+        if (string_dec s1 "$data") then
+          if (string_dec s2 "$type") then
+            match (ejson_brands j2) with
+            | Some br => dbrand br (ejson_to_data_pre j1)
+            | None => drec ((json_key_decode s1, ejson_to_data_pre j1)::(json_key_decode s2, dcoll (map ejson_to_data_pre j2))::nil)
+            end
+          else drec ((json_key_decode s1, ejson_to_data_pre j1)::(json_key_decode s2, dcoll (map ejson_to_data_pre j2))::nil)
+        else drec ((json_key_decode s1, ejson_to_data_pre j1)::(json_key_decode s2, dcoll (map ejson_to_data_pre j2))::nil)
+      | ejobject r => (drec (map (fun x => (json_key_decode (fst x), ejson_to_data_pre (snd x))) r))
+      | ejforeign fd => dforeign (foreign_to_ejson_to_data fd)
+      end.
+
+    Definition ejson_to_data h (j:ejson) :=
+      normalize_data h (ejson_to_data_pre j).
+
+  End toData.
+
+  Section toJSON.
+
+    Definition Z_to_json (n: Z) : ejson :=
+      ejbigint n.
+
+    Fixpoint data_to_ejson (d:data) : ejson :=
+      match d with
+      | dunit => ejnull
+      | dnat n => ejbigint n
+      | dfloat n => ejnumber n
+      | dbool b => ejbool b
+      | dstring s => ejstring s
+      | dcoll c => ejarray (map data_to_ejson c)
+      | drec r => ejobject (map (fun x => (json_key_encode (fst x), data_to_ejson (snd x))) r)
+      | dleft d' => ejobject (("$left"%string, data_to_ejson d')::nil)
+      | dright d' => ejobject (("$right"%string, data_to_ejson d')::nil)
+      | dbrand b d' => ejobject (("$type"%string, ejarray (map ejstring b))::("$data"%string, (data_to_ejson d'))::nil)
+      | dforeign fd => ejforeign (foreign_to_ejson_from_data fd)
+      end.
+
+  End toJSON.
+
+End DatatoEJSON.
+
+Section ModelRoundTrip.
+  Context {fdata:foreign_data}.
+  Context {ftoejson:foreign_ejson}.
+  Context {fdatatoejson:foreign_to_ejson}.
+
+  Lemma ejson_brands_map_ejstring b : ejson_brands (map ejstring b) = Some b.
+  Proof.
+    induction b; simpl; trivial.
+    now rewrite IHb.
+  Qed.
+
+  Lemma string_dec_from_neq {a b} (pf:a <> b) : exists pf2, string_dec a b = right pf2.
+  Proof.
+    destruct (string_dec a b); try congruence.
+    eauto.
+  Qed.
+
+  Ltac rewrite_string_dec_from_neq H
+    :=  let d := fresh "d" in
+        let neq := fresh "neq" in
+        destruct (string_dec_from_neq H) as [d neq]
+        ; repeat rewrite neq in *
+        ; clear d neq.
+
+  Lemma json_to_data_to_json_idempotent h d:
+    ejson_to_data h (data_to_ejson d) = normalize_data h d.
+  Proof.
+    unfold ejson_to_data.
+    induction d; simpl; trivial.
+    - f_equal.
+      repeat rewrite map_map.
+      now apply map_eq.
+    - destruct r; simpl; trivial.
+      destruct p; simpl.
+      rewrite_string_dec_from_neq (json_key_encode_not_nat s).
+      rewrite_string_dec_from_neq (json_key_encode_not_data s).
+      rewrite_string_dec_from_neq (json_key_encode_not_type s).
+      rewrite_string_dec_from_neq (json_key_encode_not_left s).
+      rewrite_string_dec_from_neq (json_key_encode_not_right s).
+      rewrite_string_dec_from_neq (json_key_encode_not_foreign s).
+
+      assert (eq_simpl: match data_to_ejson d with
+                        | ejarray j1 =>
+                          match map (fun x : string * data => (json_key_encode (fst x), data_to_ejson (snd x))) r with
+                          | nil =>
+                            drec ((json_key_decode (json_key_encode s), ejson_to_data_pre (data_to_ejson d)) :: nil)
+                          | (s2, ejnull as j2) :: nil | (s2, ejnumber _ as j2) :: nil | (s2, ejbigint _ as j2) :: nil | (s2, ejbool _ as j2) :: nil |
+                          (s2, ejstring _ as j2) :: nil | (s2, ejarray _ as j2) :: nil |
+                          (s2, ejobject _ as j2) :: nil | (s2, ejforeign _ as j2) :: nil =>
+                          drec
+                            ((json_key_decode (json_key_encode s), dcoll (map ejson_to_data_pre j1))
+                               :: (json_key_decode s2, ejson_to_data_pre j2) :: nil)
+                          | (s2, ejnull as j2) :: _ :: _ | (s2, ejnumber _ as j2) :: _ :: _ | (s2, ejbigint _ as j2) :: _ :: _ |
+                          (s2, ejbool _ as j2) :: _ :: _ | (s2, ejstring _ as j2) :: _ :: _ |
+                          (s2, ejarray _ as j2) :: _ :: _ | (s2, ejobject _ as j2) :: _ :: _ | (s2, ejforeign _ as j2) :: _ :: _ =>
+                                                           drec
+                                                             ((json_key_decode (json_key_encode s), ejson_to_data_pre (data_to_ejson d))
+                                                                :: map (fun x : string * ejson => (json_key_decode (fst x), ejson_to_data_pre (snd x)))
+                                                                (map (fun x : string * data => (json_key_encode (fst x), data_to_ejson (snd x))) r))
+                          end
+                        | _ =>
+                          match map (fun x : string * data => (json_key_encode (fst x), data_to_ejson (snd x))) r with
+                          | nil =>
+                            drec ((json_key_decode (json_key_encode s), ejson_to_data_pre (data_to_ejson d)) :: nil)
+                          | (s2, ejarray j2) :: nil =>
+                            drec
+                              ((json_key_decode (json_key_encode s), ejson_to_data_pre (data_to_ejson d))
+                                 :: (json_key_decode s2, dcoll (map ejson_to_data_pre j2)) :: nil)
+                          | (s2, ejarray j2) :: _ :: _ =>
+                            drec
+                              ((json_key_decode (json_key_encode s), ejson_to_data_pre (data_to_ejson d))
+                                 :: map (fun x : string * ejson => (json_key_decode (fst x), ejson_to_data_pre (snd x)))
+                                 (map (fun x : string * data => (json_key_encode (fst x), data_to_ejson (snd x))) r))
+                          | (s2, ejnull) :: _ | (s2, ejnumber _) :: _ | (s2, ejbigint _) :: _ | (s2, ejbool _) :: _ | 
+                          (s2, ejstring _) :: _ | (s2, ejobject _) :: _ | (s2, ejforeign _) :: _ =>
+                                                 drec
+                                                   ((json_key_decode (json_key_encode s), ejson_to_data_pre (data_to_ejson d))
+                                                      :: map (fun x : string * ejson => (json_key_decode (fst x), ejson_to_data_pre (snd x)))
+                                                      (map (fun x : string * data => (json_key_encode (fst x), data_to_ejson (snd x))) r))
+                          end
+                        end = drec ((json_key_decode (json_key_encode s), ejson_to_data_pre (data_to_ejson d))::(map (fun x : string * ejson => (json_key_decode (fst x), ejson_to_data_pre (snd x))) (map (fun x : string * data => (json_key_encode (fst x), data_to_ejson (snd x))) r)))).
+      {
+        destruct (data_to_ejson d); simpl
+        ; destruct (map (fun x : string * data => (json_key_encode (fst x), data_to_ejson (snd x))) r      ); simpl; trivial
+        ; destruct p
+        ; destruct l; simpl; trivial
+        ; destruct e; simpl; trivial
+        ; destruct l0; simpl; trivial.
+      }
+      rewrite eq_simpl; clear eq_simpl.
+      rewrite json_key_encode_decode.
+      invcs H.
+      simpl in *.
+      rewrite H2.
+      f_equal.
+      f_equal.
+      repeat rewrite map_map; simpl.
+      f_equal.
+      apply map_eq.
+      revert H3.
+      apply Forall_impl; intros.
+      rewrite json_key_encode_decode.
+      rewrite H; trivial.
+    - cut (
+          match data_to_ejson d with
+          | ejnull | _ => normalize_data h (dleft (ejson_to_data_pre (data_to_ejson d)))
+          end = dleft (normalize_data h d)).
+      + now destruct (data_to_ejson d).
+      + simpl.
+        rewrite IHd.
+        now destruct (data_to_ejson d).
+    - cut (
+          match data_to_ejson d with
+          | ejnull | _ => normalize_data h (dright (ejson_to_data_pre (data_to_ejson d)))
+          end = dright (normalize_data h d)).
+      + now destruct (data_to_ejson d).
+      + simpl.
+        rewrite IHd.
+        now destruct (data_to_ejson d).
+    - cut (
+          match data_to_ejson d with
+          | ejnull | _ =>
+                    match ejson_brands (map ejstring b) with
+                    | Some br => (normalize_data h (dbrand br (ejson_to_data_pre (data_to_ejson d))))
+                    | None =>
+                      (normalize_data h (drec
+                                           (("type"%string, dcoll (map ejson_to_data_pre (map ejstring b)))
+                                              :: ("data"%string, ejson_to_data_pre (data_to_ejson d)) :: nil)))
+                    end
+          end = dbrand (BrandRelation.canon_brands h b) (normalize_data h d)).
+      + now (destruct (data_to_ejson d); destruct (ejson_brands (map ejstring b))).
+      + simpl.
+        rewrite IHd.
+        rewrite ejson_brands_map_ejstring.
+        now destruct (data_to_ejson d).
+    - rewrite foreign_to_ejson_to_data_to_ejson.
+      reflexivity.
+  Qed.
+
+  Section RuntimeLemmas.
+    Lemma ejson_to_data_pre_jobj_nbool l b : (ejson_to_data_pre (ejobject l)) <> dbool b.
+    Proof.
+      destruct l; simpl; try congruence.
+      destruct p.
+      repeat match_destr.
+    Qed.
+
+    Lemma ejson_to_data_pre_jobj_nnat l n : (ejson_to_data_pre (ejobject l)) <> dnat n.
+    Proof.
+      destruct l; simpl; try congruence.
+      destruct p.
+      repeat match_destr.
+    Qed.
+
+    Lemma ejson_to_data_pre_jobj_nstring l s : (ejson_to_data_pre (ejobject l)) <> dstring s.
+    Proof.
+      destruct l; simpl; try congruence.
+      destruct p.
+      repeat match_destr.
+    Qed.
+
+    Lemma ejson_to_data_pre_jobj_ncoll l c : (ejson_to_data_pre (ejobject l)) <> dcoll c.
+    Proof.
+      destruct l; simpl; try congruence.
+      destruct p.
+      repeat match_destr.
+    Qed.
+
+    Lemma ejson_to_data_object_not_boolean h l b:
+      ~(ejson_to_data h (ejobject l) = dbool b).
+    Proof.
+      unfold ejson_to_data.
+      apply normalize_data_forall_ndbool.
+      apply ejson_to_data_pre_jobj_nbool.
+    Qed.
+
+    Lemma ejson_to_data_object_not_nat h l n:
+      ~(ejson_to_data h (ejobject l) = dnat n).
+    Proof.
+      unfold ejson_to_data.
+      apply normalize_data_forall_ndnat.
+      apply ejson_to_data_pre_jobj_nnat.
+    Qed.
+
+    Lemma ejson_to_data_object_not_string h l b:
+      ~(ejson_to_data h (ejobject l) = dstring b).
+    Proof.
+      unfold ejson_to_data.
+      apply normalize_data_forall_ndstring.
+      apply ejson_to_data_pre_jobj_nstring.
+    Qed.
+
+    Lemma ejson_to_data_object_not_coll h l j:
+      ~(ejson_to_data h (ejobject l) = dcoll j).
+    Proof.
+      unfold ejson_to_data.
+      apply normalize_data_forall_ndcoll.
+      apply ejson_to_data_pre_jobj_ncoll.
+    Qed.
+
+    Lemma rec_ejson_key_encode_roundtrip h s i0:
+      drec ((s, ejson_to_data h i0)::nil) = ejson_to_data h (ejobject ((json_key_encode s, i0)::nil)).
+    Proof.
+      unfold ejson_to_data; simpl.
+      rewrite_string_dec_from_neq (json_key_encode_not_left s).
+      rewrite_string_dec_from_neq (json_key_encode_not_right s).
+      rewrite_string_dec_from_neq (json_key_encode_not_foreign s).
+      rewrite json_key_encode_decode.
+      now destruct i0.
+    Qed.
+
+    (* XXX Some assumptions for the correctness of operators translation -- they do not hold as-is *)
+
+    Lemma assoc_lookupr_json_key_encode_roundtrip h l s:
+      match ejson_to_data h (ejobject l) with
+      | drec r => assoc_lookupr ODT_eqdec r s
+      | _ => None
+      end =
+      match assoc_lookupr ODT_eqdec l (json_key_encode s) with
+      | Some a' => Some (ejson_to_data h a')
+      | None => None
+      end.
+    Proof.
+      admit.
+    Admitted.
+
+    Lemma rremove_json_key_encode_roundtrip h l s:
+      match ejson_to_data h (ejobject l) with
+      | drec r => Some (drec (rremove r s))
+      | _ => None
+      end = Some (ejson_to_data h (ejobject (rremove l (json_key_encode s)))).
+    Proof.
+      
+      admit.
+    Admitted.
+
+  End RuntimeLemmas.
+End ModelRoundTrip.
