compiler/src/Common/EJSON/EJSON.v
@@ -1,0 +1,239 @@
+(*
+ * Copyright 2015-2016 IBM Corporation
+ *
+ * Licensed under the Apache License, Version 2.0 (the "License");
+ * you may not use this file except in compliance with the License.
+ * You may obtain a copy of the License at
+ *
+ * http://www.apache.org/licenses/LICENSE-2.0
+ *
+ * Unless required by applicable law or agreed to in writing, software
+ * distributed under the License is distributed on an "AS IS" BASIS,
+ * WITHOUT WARRANTIES OR CONDITIONS OF ANY KIND, either express or implied.
+ * See the License for the specific language governing permissions and
+ * limitations under the License.
+ *)
+
+Require Import List.
+Require Import Ascii.
+Require Import String.
+Require Import ZArith.
+Require Import Bool.
+Require Import JsAst.JsNumber.
+Require Import Float.
+Require Import ToString.
+Require Import CoqLibAdd.
+Require Import StringAdd.
+Require Import Digits.
+Require Import EquivDec.
+Require Import ForeignEJSON.
+Require Import Utils.
+
+Section EJSON.
+  Context {fejson:foreign_ejson}.
+
+  Unset Elimination Schemes.
+
+  Inductive ejson : Set :=
+  | ejnull : ejson
+  | ejnumber : float -> ejson
+  | ejbigint : Z -> ejson
+  | ejbool : bool -> ejson
+  | ejstring : string -> ejson
+  | ejarray : list ejson -> ejson
+  | ejobject : list (string * ejson) -> ejson
+  | ejforeign : foreign_ejson_type -> ejson
+  .
+
+  Set Elimination Schemes.
+
+  (** Induction principles used as backbone for inductive proofs on json *)
+  Definition ejson_rect (P : ejson -> Type)
+             (fnull : P ejnull)
+             (fnumber : forall n : number, P (ejnumber n))
+             (fbigint : forall n : Z, P (ejbigint n))
+             (fbool : forall b : bool, P (ejbool b))
+             (fstring : forall s : string, P (ejstring s))
+             (farray : forall c : list ejson, Forallt P c -> P (ejarray c))
+             (fobject : forall r : list (string * ejson), Forallt (fun ab => P (snd ab)) r -> P (ejobject r))
+             (fforeign: forall fd, P (ejforeign fd))
+    :=
+      fix F (j : ejson) : P j :=
+    match j as j0 return (P j0) with
+      | ejnull => fnull
+      | ejnumber x => fnumber x
+      | ejbigint x => fbigint x
+      | ejbool x => fbool x
+      | ejstring x => fstring x
+      | ejarray x => farray x ((fix F2 (c : list ejson) : Forallt P c :=
+                            match c as c0 with
+                              | nil => Forallt_nil _
+                              | cons j c0 => @Forallt_cons _ P j c0 (F j) (F2 c0)
+                            end) x)
+      | ejobject x => fobject x ((fix F3 (r : list (string*ejson)) : Forallt (fun ab => P (snd ab)) r :=
+                           match r as c0 with
+                             | nil => Forallt_nil _
+                             | cons sj c0 => @Forallt_cons _ (fun ab => P (snd ab)) sj c0 (F (snd sj)) (F3 c0)
+                           end) x)
+      | ejforeign fd => fforeign fd
+    end.
+
+  Definition ejson_ind (P : ejson -> Prop)
+             (fnull : P ejnull)
+             (fnumber : forall n : number, P (ejnumber n))
+             (fbigint : forall n : Z, P (ejbigint n))
+             (fbool : forall b : bool, P (ejbool b))
+             (fstring : forall s : string, P (ejstring s))
+             (farray : forall c : list ejson, Forall P c -> P (ejarray c))
+             (fobject : forall r : list (string * ejson), Forall (fun ab => P (snd ab)) r -> P (ejobject r))
+             (fforeign: forall fd, P (ejforeign fd))
+    :=
+      fix F (j : ejson) : P j :=
+    match j as j0 return (P j0) with
+      | ejnull => fnull
+      | ejnumber x => fnumber x
+      | ejbigint x => fbigint x
+      | ejbool x => fbool x
+      | ejstring x => fstring x
+      | ejarray x => farray x ((fix F2 (c : list ejson) : Forall P c :=
+                            match c with
+                              | nil => Forall_nil _
+                              | cons j c0 => @Forall_cons _ P j c0 (F j) (F2 c0)
+                            end) x)
+      | ejobject x => fobject x ((fix F3 (r : list (string*ejson)) : Forall (fun ab => P (snd ab)) r :=
+                           match r with
+                             | nil => Forall_nil _
+                             | cons sj c0 => @Forall_cons _ (fun ab => P (snd ab)) sj c0 (F (snd sj)) (F3 c0)
+                           end) x)
+      | ejforeign fd => fforeign fd
+    end.
+
+  Definition ejson_rec (P:ejson->Set) := ejson_rect P.
+
+  Lemma ejsonInd2 (P : ejson -> Prop)
+        (f : P ejnull)
+        (f0 : forall n : number, P (ejnumber n))
+        (f1 : forall n : Z, P (ejbigint n))
+        (f2 : forall b : bool, P (ejbool b))
+        (f3 : forall s : string, P (ejstring s))
+        (f4 : forall c : list ejson, (forall x, In x c -> P x) -> P (ejarray c))
+        (f5 : forall r : list (string * ejson), (forall x y, In (x,y) r -> P y) -> P (ejobject r))
+        (fforeign : forall fd, P (ejforeign fd)):
+    forall d, P d.
+  Proof.
+    intros.
+    apply ejson_ind; trivial.
+    - intros. rewrite Forall_forall in H.
+      auto.
+    - intros. rewrite Forall_forall in H.
+      apply f5.
+      intros. apply (H (x,y)). trivial.
+  Qed.
+
+  (** Equality is decidable for json *)
+  Lemma ejson_eq_dec : forall x y:ejson, {x=y}+{x<>y}.
+  Proof.
+    induction x; destruct y; try solve[right; inversion 1].
+    - left; trivial.
+    - destruct (float_eq_dec n f).
+      + left; f_equal; trivial.
+      + right;intro;apply c;inversion H; reflexivity.
+    - destruct (Z.eq_dec n z).
+      + left; f_equal; trivial.
+      + right;intro;apply n0;inversion H; trivial.
+    - destruct (bool_dec b b0).
+      + left; f_equal; trivial.
+      + right;intro;apply n;inversion H; trivial. 
+    - destruct (string_dec s s0).
+      + left; f_equal; trivial.
+      + right;intro;apply n;inversion H; trivial.
+    - destruct (list_Forallt_eq_dec c l H). subst. auto.
+      right; inversion 1. auto.
+    - destruct (list_Forallt_eq_dec r l); subst; auto.
+      + apply (forallt_impl H).
+        apply forallt_weaken; clear; intros.
+        destruct x; destruct y; simpl in *.
+        apply pair_eq_dec; auto.
+        apply string_dec.
+      + right; inversion 1; auto.
+    - destruct (foreign_ejson_dec fd f).
+      + left. f_equal; apply e.
+      + right. inversion 1; congruence.
+  Defined.
+
+  (* begin hide *)
+  Global Instance ejson_eqdec : EqDec ejson eq := ejson_eq_dec.
+  (* begin hide *)
+
+  Section toString.
+
+    Local Open Scope string.
+
+    Fixpoint ejsonStringify (quotel:string) (j : ejson) : string
+      := match j with
+         | ejnull => "null"
+         | ejnumber n => toString n
+         | ejbigint n => toString n
+         | ejbool b => toString b
+         | ejstring s => stringToStringQuote quotel s
+         | ejarray ls =>
+           let ss := map (ejsonStringify quotel) ls in
+           "[" ++ (concat ", " ss) ++ "]"
+         | ejobject ls =>
+           let ss := (map (fun kv =>
+                             let '(k,v) := kv in
+                             "" ++ quotel ++ "" ++ k ++ ""
+                                ++ quotel ++ ": " ++ (ejsonStringify quotel v)) ls)
+           in "{" ++ (concat ", " ss) ++ "}"
+         | ejforeign fd => toString fd
+         end.
+
+  End toString.
+
+  Section preProcess.
+    Fixpoint json_to_ejson (j:json) : ejson :=
+      match j with
+      | jnull => ejnull
+      | jnumber n => ejnumber n
+      | jbool b => ejbool b
+      | jstring s => ejstring s
+      | jarray c => ejarray (map json_to_ejson c)
+      | jobject nil => ejobject nil
+      | jobject ((s1,j')::nil) =>
+        if (string_dec s1 "$nat") then
+          match j' with
+          | jnumber n => ejbigint (float_truncate n)
+          | _ => ejobject ((json_key_decode s1, json_to_ejson j')::nil)
+          end
+        else
+          if (string_dec s1 "$foreign") then
+            match foreign_ejson_from_json j' with
+            | Some fd => ejforeign fd
+            | None => ejobject ((json_key_decode s1, json_to_ejson j')::nil)
+            end
+          else ejobject ((s1, json_to_ejson j')::nil)
+      | jobject r => ejobject (map (fun x => (fst x, json_to_ejson (snd x))) r)
+      end.
+
+    Fixpoint ejson_to_json (j:ejson) : json :=
+      match j with
+      | ejnull => jnull
+      | ejnumber n => jnumber n
+      | ejbigint n => jnumber (float_of_int n)
+      | ejbool b => jbool b
+      | ejstring s => jstring s
+      | ejarray c => jarray (map ejson_to_json c)
+      | ejobject nil => jobject nil
+      | ejobject ((s1,j')::nil) =>
+        if (string_dec s1 "$nat") then
+          match j' with
+          | ejbigint n => jobject ((s1, jnumber (float_of_int n))::nil)
+          | _ => jobject ((s1, ejson_to_json j')::nil)
+          end
+        else jobject ((s1, ejson_to_json j')::nil)
+      | ejobject r => jobject (map (fun x => (fst x, ejson_to_json (snd x))) r)
+      | ejforeign fd => jobject (("$foreign"%string, foreign_ejson_to_json fd)::nil)
+      end.
+
+  End preProcess.
+End EJSON.
