compiler/src/Common/EJSON/EJSONOperators.v
@@ -1,0 +1,198 @@
+(*
+ * Copyright 2015-2018 Clause
+ *
+ * Licensed under the Apache License, Version 2.0 (the "License");
+ * you may not use this file except in compliance with the License.
+ * You may obtain a copy of the License at
+ *
+ * http://www.apache.org/licenses/LICENSE-2.0
+ *
+ * Unless required by applicable law or agreed to in writing, software
+ * distributed under the License is distributed on an "AS IS" BASIS,
+ * WITHOUT WARRANTIES OR CONDITIONS OF ANY KIND, either express or implied.
+ * See the License for the specific language governing permissions and
+ * limitations under the License.
+ *)
+
+(* Unary operators *)
+
+Require Import String.
+Require Import List.
+Require Import ZArith.
+Require Import Float.
+Require Import ListAdd.
+Require Import Lift.
+Require Import Assoc.
+Require Import Bindings.
+Require Import ForeignEJSON.
+Require Import EJSON.
+
+Section EJSONOperators.
+
+  Import ListNotations.
+
+  Inductive ejson_op :=     (* XXX TODO XXX *)(* JsAst *)                     (* Syntax *)
+  | EJSONOpNot : ejson_op                          (* unary_op_not *)              (* !v *)
+  | EJSONOpNeg : ejson_op                          (* unary_op_neg *)              (* -v *)
+  | EJSONOpAnd : ejson_op                          (* binary_op_and *)             (* v1 && v2 *)
+  | EJSONOpOr : ejson_op                           (* binary_op_or *)              (* v1 || v2 *)
+  | EJSONOpLt : ejson_op                           (* binary_op_lt *)              (* v1 < v2 *)
+  | EJSONOpLe : ejson_op                           (* binary_op_le *)              (* v1 <= v2 *)
+  | EJSONOpGt : ejson_op                           (* binary_op_gt *)              (* v1 > v2 *)
+  | EJSONOpGe : ejson_op                           (* binary_op_ge *)              (* v1 >= v2 *)
+  | EJSONOpAddString : ejson_op                    (* binary_op_add *)             (* v1 + v2 *)
+  | EJSONOpAddNumber : ejson_op                    (* binary_op_add *)             (* v1 + v2 *)
+  | EJSONOpSub : ejson_op                          (* binary_op_sub *)             (* v1 - v2 *)
+  | EJSONOpMult : ejson_op                         (* binary_op_mult *)            (* v1 * v2 *)
+  | EJSONOpDiv : ejson_op                          (* binary_op_div *)             (* v1 / v2 *)
+  | EJSONOpStrictEqual : ejson_op                  (* binary_op_strict_equal *)    (* v1 === v2 *)
+  | EJSONOpStrictDisequal : ejson_op               (* binary_op_strict_disequal *) (* v1 !== v2 *)
+  (*| EJSONOpIn : ejson_op *)                        (* binary_op_in *)              (* v1 in v2 *) (* XXX either 'in' or hasOwnProperty, not both *)
+  (* Array Stuff *)
+  | EJSONOpArray : ejson_op                        (* expr_array *)                (* [ v1, ...vn ] XXX Nary? *)
+  | EJSONOpArrayLength : ejson_op                  (* expr_access? *)              (* v.length *)
+  | EJSONOpArrayPush : ejson_op                    (* expr_access? *)              (* v.push(v2) or var v' = v.slice(); v'.push(v2) XXX Does not actually claim to be mutable from a semantic stand-point *)
+  | EJSONOpArrayAccess : ejson_op                  (* array_get *)                 (* v[i] *)
+  (* Object Stuff *)
+  | EJSONOpObject : list string -> ejson_op        (* expr_object *)               (* { a1:v1, ...an:vn } XXX Nary? *)
+  | EJSONOpAccess : string -> ejson_op             (* expr_access *)               (* v['a'] or v.a *)
+  | EJSONOpHasOwnProperty : string -> ejson_op     (* expr_call ?? XXX *)          (* v.hasOwnProperty('a') *)
+  | EJSONOpToString : ejson_op                     (* expr_call ?? XXX *)          (* v.toString() *)
+  (* Math stuff *)
+  | EJSONOpMathMin : ejson_op                      (* expr_call *)                 (* Math.min(e1, e2) *)
+  | EJSONOpMathMax : ejson_op                      (* expr_call *)                 (* Math.max(e1, e2) *)
+  | EJSONOpMathMinApply : ejson_op                 (* expr_call *)                 (* Math.min.apply(Math, e) *)
+  | EJSONOpMathMaxApply : ejson_op                 (* expr_call *)                 (* Math.max.apply(Math, e) *)
+  | EJSONOpMathPow : ejson_op                      (* expr_call *)                 (* Math.pow(e1, e2) *)
+  | EJSONOpMathExp : ejson_op                      (* expr_call *)                 (* Math.exp(e) *)
+  | EJSONOpMathAbs : ejson_op                      (* expr_call *)                 (* Math.abs(e) *)
+  | EJSONOpMathLog : ejson_op                      (* expr_call *)                 (* Math.log2(e) *)
+  | EJSONOpMathLog10 : ejson_op                    (* expr_call *)                 (* Math.log10(e) *)
+  | EJSONOpMathSqrt : ejson_op                     (* expr_call *)                 (* Math.sqrt(e) *)
+  | EJSONOpMathCeil : ejson_op                     (* expr_call *)                 (* Math.ceil(e) *)
+  | EJSONOpMathFloor : ejson_op                    (* expr_call *)                 (* Math.floor(e) *)
+  | EJSONOpMathTrunc : ejson_op                    (* expr_call *)                 (* Math.trunc(e) *)
+  .
+
+  Section Evaluation.
+    Context {fejson:foreign_ejson}.
+
+    Definition ejson_op_eval (op:ejson_op) (j:list ejson) : option ejson :=
+      match op with
+      | EJSONOpNot =>
+        match j with
+        | [ejbool b] => Some (ejbool (negb b))
+        | _ => None
+        end
+      | EJSONOpNeg =>
+        match j with
+        | [ejnumber n] => Some (ejnumber (float_neg n))
+        | _ => None
+        end
+      | EJSONOpAnd =>
+        match j with
+        | [ejbool b1; ejbool b2] => Some (ejbool (andb b1 b2))
+        | _ => None
+        end
+      | EJSONOpOr =>
+        match j with
+        | [ejbool b1; ejbool b2] => Some (ejbool (orb b1 b2))
+        | _ => None
+        end
+      | EJSONOpLt =>
+        match j with
+        | [ejnumber n1; ejnumber n2] => Some (ejbool (float_lt n1 n2))
+        | _ => None
+        end
+      | EJSONOpLe =>
+        match j with
+        | [ejnumber n1; ejnumber n2] => Some (ejbool (float_le n1 n2))
+        | _ => None
+        end
+      | EJSONOpGt =>
+        match j with
+        | [ejnumber n1; ejnumber n2] => Some (ejbool (float_gt n1 n2))
+        | _ => None
+        end
+      | EJSONOpGe =>
+        match j with
+        | [ejnumber n1; ejnumber n2] => Some (ejbool (float_ge n1 n2))
+        | _ => None
+        end
+      | EJSONOpAddString =>
+        match j with
+        | [ejstring s1; ejstring s2] => Some (ejstring (s1 ++ s2))
+        | _ => None
+        end
+      | EJSONOpAddNumber =>
+        match j with
+        | [ejnumber n1; ejnumber n2] => Some (ejnumber (float_add n1 n2))
+        | _ => None
+        end
+      | EJSONOpSub =>
+        match j with
+        | [ejnumber n1; ejnumber n2] => Some (ejnumber (float_sub n1 n2))
+        | _ => None
+        end
+      | EJSONOpMult =>
+        match j with
+        | [ejnumber n1; ejnumber n2] => Some (ejnumber (float_mult n1 n2))
+        | _ => None
+        end
+      | EJSONOpDiv =>
+        match j with
+        | [ejnumber n1; ejnumber n2] => Some (ejnumber (float_div n1 n2))
+        | _ => None
+        end
+      | EJSONOpStrictEqual => None (* XXX TODO *)
+      | EJSONOpStrictDisequal => None (* XXX TODO *)
+      | EJSONOpArray => Some (ejarray j)
+      | EJSONOpArrayLength =>
+        match j with
+        | [ejarray ja] => Some (ejnumber (float_of_int (Z_of_nat (List.length ja))))
+        | _ => None
+        end
+      | EJSONOpArrayPush =>
+        match j with
+        | [ejarray ja; je] => Some (ejarray (ja ++ [je]))
+        | _ => None
+        end
+      | EJSONOpArrayAccess =>
+        match j with
+        | [ejarray ja; ejnumber n] => None (* XXX TODO XXX *)
+        | _ => None
+        end
+      | EJSONOpObject atts =>
+        lift ejobject (zip atts j)
+      | EJSONOpAccess att =>
+        match j with
+        | [ejobject jl] =>
+          edot jl att
+        | _ => None
+        end
+      | EJSONOpHasOwnProperty a =>
+        match j  with
+        | [ejobject jl] =>
+          if in_dec string_dec a (domain jl)
+          then Some (ejbool true)
+          else Some (ejbool false)
+        | _ => None
+        end
+      | EJSONOpToString => None (* XXX TODO XXX *)
+      | EJSONOpMathMin => None (* XXX TODO XXX *)
+      | EJSONOpMathMax => None (* XXX TODO XXX *)
+      | EJSONOpMathMinApply => None (* XXX TODO XXX *)
+      | EJSONOpMathMaxApply => None (* XXX TODO XXX *)
+      | EJSONOpMathExp => None (* XXX TODO XXX *)
+      | EJSONOpMathPow => None (* XXX TODO XXX *)
+      | EJSONOpMathAbs => None (* XXX TODO XXX *)
+      | EJSONOpMathLog => None (* XXX TODO XXX *)
+      | EJSONOpMathLog10 => None (* XXX TODO XXX *)
+      | EJSONOpMathSqrt => None (* XXX TODO XXX *)
+      | EJSONOpMathCeil => None (* XXX TODO XXX *)
+      | EJSONOpMathFloor => None (* XXX TODO XXX *)
+      | EJSONOpMathTrunc => None (* XXX TODO XXX *)
+      end.
+  End Evaluation.
+
+End EJSONOperators.
