compiler/src/Compiler/Model/TrivialModel.v
@@ -22,8 +22,9 @@ Require Import CommonSystem.
 Require Import ForeignToJava.
 Require Import ForeignToJavaScript.
 Require Import ForeignToJavaScriptAst.
+Require Import ForeignEJSONtoJavaScriptAst.
 Require Import ForeignToScala.
-Require Import ForeignDataToJSON.
+Require Import ForeignDataToEJSON.
 Require Import ForeignTypeToJSON.
 Require Import ForeignReduceOps.
 Require Import ForeignToReduceOps.
@@ -44,7 +45,7 @@ Require Import Dataframe.
 Program Instance trivial_foreign_data : foreign_data
   := mk_foreign_data Empty_set _ _ _ _ _ _.
 Next Obligation.
-  intros []. 
+  intros [].
 Defined.
 Next Obligation.
   destruct a.
@@ -54,6 +55,30 @@ Next Obligation.
 Defined.
 Next Obligation.
   constructor; intros [].
+Defined.
+
+Program Instance trivial_foreign_ejson : foreign_ejson
+  := mk_foreign_ejson Empty_set _ _ _ _ _ _ _ _ _.
+Next Obligation.
+  intros [].
+Defined.
+Next Obligation.
+  destruct a.
+Defined.
+Next Obligation.
+  destruct a.
+Defined.
+Next Obligation.
+  constructor; intros [].
+Defined.
+Next Obligation.
+  exact None.
+Defined.
+Next Obligation.
+  exact jnull.
+Defined.
+Next Obligation.
+  destruct fd.
 Defined.
 
 Program Instance trivial_foreign_unary_op:
@@ -90,150 +115,141 @@ Next Obligation.
   destruct op. 
 Defined.
 
-  Program Instance trivial_foreign_to_JSON : foreign_to_JSON
-    := mk_foreign_to_JSON trivial_foreign_data _ _ _.
-  Next Obligation.
-    exact None.
-  Defined.
-  Next Obligation.
-     destruct fd. 
-  Defined.
-  Next Obligation.
-    destruct fd.
-  Qed.
-  
-  Instance trivial_foreign_runtime :
-    foreign_runtime
+Program Instance trivial_foreign_to_ejson : foreign_to_ejson
+  := mk_foreign_to_ejson trivial_foreign_ejson trivial_foreign_data _ _ _.
+
+Instance trivial_foreign_runtime :
+  foreign_runtime
   := mk_foreign_runtime
+       trivial_foreign_ejson
        trivial_foreign_data
        trivial_foreign_unary_op
        trivial_foreign_binary_op
-       trivial_foreign_to_JSON.
+       trivial_foreign_to_ejson.
 
-  Program Instance trivial_foreign_type : foreign_type
-    := mk_foreign_type Empty_set _ _ _ _ _ _ _.
-  Next Obligation.
-     intros []. 
-  Defined.
-  Next Obligation.
-    econstructor;
-      intros [].
-    Grab Existential Variables.
-    solve [intros []].
-    solve [intros []].
-  Defined.
-  Next Obligation.
-    destruct a.
-  Defined.
-  Next Obligation.
-    destruct a.
-  Defined.
-  Next Obligation.
-    constructor;
-      intros [].
-  Defined.
-  Next Obligation.
+Program Instance trivial_foreign_type : foreign_type
+  := mk_foreign_type Empty_set _ _ _ _ _ _ _.
+Next Obligation.
+  intros []. 
+Defined.
+Next Obligation.
+  econstructor;
     intros [].
-  Defined.
-  Next Obligation.
-    econstructor;
-      intros [].
-  Defined.
+  Grab Existential Variables.
+  solve [intros []].
+  solve [intros []].
+Defined.
+Next Obligation.
+  destruct a.
+Defined.
+Next Obligation.
+  destruct a.
+Defined.
+Next Obligation.
+  constructor;
+    intros [].
+Defined.
+Next Obligation.
+  intros [].
+Defined.
+Next Obligation.
+  econstructor;
+    intros [].
+Defined.
 
-  Program Instance trivial_foreign_data_typing :
-    @foreign_data_typing trivial_foreign_data trivial_foreign_type
-    := mk_foreign_data_typing
-         trivial_foreign_data
-         trivial_foreign_type
-         _ _ _ _ _ _ _ _.
-  Next Obligation.
-    destruct d.
-  Defined.
-  Next Obligation.
-    destruct d.
-  Defined.
-  Next Obligation.
-    destruct d.
-  Defined.
-  Next Obligation.
-    destruct d.
-  Defined.
-  Next Obligation.
-    destruct d.
-  Defined.
+Program Instance trivial_foreign_data_typing :
+  @foreign_data_typing trivial_foreign_data trivial_foreign_type
+  := mk_foreign_data_typing
+       trivial_foreign_data
+       trivial_foreign_type
+       _ _ _ _ _ _ _ _.
+Next Obligation.
+  destruct d.
+Defined.
+Next Obligation.
+  destruct d.
+Defined.
+Next Obligation.
+  destruct d.
+Defined.
+Next Obligation.
+  destruct d.
+Defined.
+Next Obligation.
+  destruct d.
+Defined.
 
-  Program Instance trivial_foreign_unary_op_typing
-          {model:brand_model} :
-    @foreign_unary_op_typing
-      trivial_foreign_data
-      trivial_foreign_unary_op
-      trivial_foreign_type
-      trivial_foreign_data_typing
-      model
-    := mk_foreign_unary_op_typing
-         _ _ _ _ _ _
-         _ _ _ _ _ _.
-  Next Obligation.
-    destruct fu.
-  Defined.
-  Next Obligation.
-    destruct fu.
-  Defined.
-  Next Obligation.
-    destruct fu.
-  Defined.
-  Next Obligation.
-    destruct fu.
-  Defined.
-  Next Obligation.
-    destruct fu.
-  Defined.
-  Next Obligation.
-    destruct fu.
-  Defined.
-  Next Obligation.
-    destruct fu.
-  Defined.
-  
+Program Instance trivial_foreign_unary_op_typing
+        {model:brand_model} :
+  @foreign_unary_op_typing
+    trivial_foreign_data
+    trivial_foreign_unary_op
+    trivial_foreign_type
+    trivial_foreign_data_typing
+    model
+  := mk_foreign_unary_op_typing
+       _ _ _ _ _ _
+       _ _ _ _ _ _.
+Next Obligation.
+  destruct fu.
+Defined.
+Next Obligation.
+  destruct fu.
+Defined.
+Next Obligation.
+  destruct fu.
+Defined.
+Next Obligation.
+  destruct fu.
+Defined.
+Next Obligation.
+  destruct fu.
+Defined.
+Next Obligation.
+  destruct fu.
+Defined.
+Next Obligation.
+  destruct fu.
+Defined.
 
-  Program Instance trivial_foreign_binary_op_typing
-          {model:brand_model} :
-    @foreign_binary_op_typing
-      trivial_foreign_data
-      trivial_foreign_binary_op
-      trivial_foreign_type
-      trivial_foreign_data_typing
-      model
-    := mk_foreign_binary_op_typing
-         _ _ _ _ _ _
-         _ _ _ _ _ _.
-  Next Obligation.
-    destruct fb.
-  Defined.
-  Next Obligation.
-    destruct fb.
-  Defined.
-  Next Obligation.
-    destruct fb.
-  Defined.
-  Next Obligation.
-    destruct fb.
-  Defined.
-  Next Obligation.
-    destruct fb.
-  Defined.
-  Next Obligation.
-    destruct fb.
-  Defined.
-  Next Obligation.
-    destruct fb.
-  Defined.
+Program Instance trivial_foreign_binary_op_typing
+        {model:brand_model} :
+  @foreign_binary_op_typing
+    trivial_foreign_data
+    trivial_foreign_binary_op
+    trivial_foreign_type
+    trivial_foreign_data_typing
+    model
+  := mk_foreign_binary_op_typing
+       _ _ _ _ _ _
+       _ _ _ _ _ _.
+Next Obligation.
+  destruct fb.
+Defined.
+Next Obligation.
+  destruct fb.
+Defined.
+Next Obligation.
+  destruct fb.
+Defined.
+Next Obligation.
+  destruct fb.
+Defined.
+Next Obligation.
+  destruct fb.
+Defined.
+Next Obligation.
+  destruct fb.
+Defined.
+Next Obligation.
+  destruct fb.
+Defined.
 
-  Instance trivial_foreign_typing {model:brand_model}:
-    @foreign_typing
-      trivial_foreign_runtime
-      trivial_foreign_type
-      model
+Instance trivial_foreign_typing {model:brand_model}:
+  @foreign_typing
+    trivial_foreign_runtime
+    trivial_foreign_type
+    model
   := mk_foreign_typing
        trivial_foreign_runtime
        trivial_foreign_type
@@ -242,167 +258,179 @@ Defined.
        trivial_foreign_unary_op_typing
        trivial_foreign_binary_op_typing.
 
-  Instance trivial_basic_model {model:brand_model} :
-    basic_model
-    := mk_basic_model
-         trivial_foreign_runtime
-         trivial_foreign_type
-         model
-         trivial_foreign_typing.
+Instance trivial_basic_model {model:brand_model} :
+  basic_model
+  := mk_basic_model
+       trivial_foreign_runtime
+       trivial_foreign_type
+       model
+       trivial_foreign_typing.
 
-  Program Instance trivial_foreign_to_java :
-    @foreign_to_java trivial_foreign_runtime
-    := mk_foreign_to_java
-         trivial_foreign_runtime
-         _ _ _.
-  Next Obligation.
-    destruct fd.
-  Defined.
+Program Instance trivial_foreign_to_java :
+  @foreign_to_java trivial_foreign_runtime
+  := mk_foreign_to_java
+       trivial_foreign_runtime
+       _ _ _.
+Next Obligation.
+  destruct fd.
+Defined.
 
-  Program Instance trivial_foreign_to_javascript :
-    @foreign_to_javascript trivial_foreign_runtime
-    := mk_foreign_to_javascript
-         trivial_foreign_runtime
-         _ _.
+Program Instance trivial_foreign_to_javascript :
+  @foreign_to_javascript trivial_foreign_runtime
+  := mk_foreign_to_javascript
+       trivial_foreign_runtime
+       _ _.
 
-  Program Instance trivial_foreign_to_ajavascript :
-    @foreign_to_ajavascript trivial_foreign_runtime
-    := mk_foreign_to_ajavascript
-         trivial_foreign_runtime
-         _ _.
+Program Instance trivial_foreign_to_ajavascript :
+  @foreign_to_ajavascript trivial_foreign_runtime
+  := mk_foreign_to_ajavascript
+       trivial_foreign_runtime
+       _ _.
 
-  Program Instance trivial_foreign_to_scala :
-    @foreign_to_scala trivial_foreign_runtime trivial_foreign_type
-    := mk_foreign_to_scala
-         trivial_foreign_runtime trivial_foreign_type
-         _ _.
-  Next Obligation.
-    exact "TRIVIAL MODEL DOES NOT SUPPORT FOREIGN TYPES"%string.
-  Defined.
-  
-  Program Instance trivial_foreign_type_to_JSON : foreign_type_to_JSON
-    := mk_foreign_type_to_JSON trivial_foreign_type _ _.
-  Next Obligation.
-    exact None.
-  Defined.
-  Next Obligation.
-     destruct fd. 
-  Defined.
+Program Instance trivial_foreign_ejson_to_ajavascript :
+  @foreign_ejson_to_ajavascript trivial_foreign_ejson
+  := mk_foreign_ejson_to_ajavascript
+       trivial_foreign_ejson
+       _.
+Next Obligation.
+  destruct fe.
+Defined.
 
-  Program Instance trivial_foreign_reduce_op
-            {fdata:foreign_data}:
-      foreign_reduce_op
-    := mk_foreign_reduce_op fdata Empty_set _ _ _ _.
-  Next Obligation.
-     intros []. 
-  Defined.
-  Next Obligation.
-    constructor.
-    intros []. 
-  Defined.
-  Next Obligation.
-    destruct op. 
-  Defined.
-  Next Obligation.
-    destruct op. 
-  Defined.
+Program Instance trivial_foreign_to_scala :
+  @foreign_to_scala trivial_foreign_runtime trivial_foreign_type
+  := mk_foreign_to_scala
+       trivial_foreign_runtime trivial_foreign_type
+       _ _.
+Next Obligation.
+  exact "TRIVIAL MODEL DOES NOT SUPPORT FOREIGN TYPES"%string.
+Defined.
 
-  Program Instance trivial_foreign_to_reduce_op :
-      foreign_to_reduce_op
-    := mk_foreign_to_reduce_op trivial_foreign_runtime trivial_foreign_reduce_op _ _ _ _.
-  Next Obligation.
-    exact None.
-  Defined.
-  Next Obligation.
-    exact None.
-  Defined.
+Program Instance trivial_foreign_type_to_JSON : foreign_type_to_JSON
+  := mk_foreign_type_to_JSON trivial_foreign_type _ _.
+Next Obligation.
+  exact None.
+Defined.
+Next Obligation.
+  destruct fd. 
+Defined.
 
-  Program Instance trivial_foreign_to_spark : foreign_to_spark
+Program Instance trivial_foreign_reduce_op
+        {fdata:foreign_data}:
+  foreign_reduce_op
+  := mk_foreign_reduce_op fdata Empty_set _ _ _ _.
+Next Obligation.
+  intros []. 
+Defined.
+Next Obligation.
+  constructor.
+  intros []. 
+Defined.
+Next Obligation.
+  destruct op. 
+Defined.
+Next Obligation.
+  destruct op. 
+Defined.
+
+Program Instance trivial_foreign_to_reduce_op :
+  foreign_to_reduce_op
+  := mk_foreign_to_reduce_op trivial_foreign_runtime trivial_foreign_reduce_op _ _ _ _.
+Next Obligation.
+  exact None.
+Defined.
+Next Obligation.
+  exact None.
+Defined.
+
+Program Instance trivial_foreign_to_spark : foreign_to_spark
   := mk_foreign_to_spark trivial_foreign_runtime trivial_foreign_reduce_op _ _.
 
 Existing Instance silent_optimizer_logger.
 
-  Module TrivialRuntime <: CompilerRuntime.
-    Definition compiler_foreign_type : foreign_type
-      := trivial_foreign_type.
-    Definition compiler_foreign_runtime : foreign_runtime
-      := trivial_foreign_runtime.
-    Definition compiler_foreign_to_java : foreign_to_java
-      := trivial_foreign_to_java.
-    Definition compiler_foreign_to_javascript : foreign_to_javascript
-      := trivial_foreign_to_javascript.
-    Definition compiler_foreign_to_ajavascript : foreign_to_ajavascript
-      := trivial_foreign_to_ajavascript.
-    Definition compiler_foreign_to_scala : foreign_to_scala
-      := trivial_foreign_to_scala.
-    Definition compiler_foreign_to_JSON : foreign_to_JSON
-      := trivial_foreign_to_JSON.
-    Definition compiler_foreign_type_to_JSON : foreign_type_to_JSON
-      := trivial_foreign_type_to_JSON.
-    Definition compiler_foreign_reduce_op : foreign_reduce_op
-      := trivial_foreign_reduce_op.
-    Definition compiler_foreign_to_reduce_op : foreign_to_reduce_op
-      := trivial_foreign_to_reduce_op.
-    Definition compiler_foreign_to_spark : foreign_to_spark
-      := trivial_foreign_to_spark.
-    Definition compiler_nraenv_optimizer_logger : optimizer_logger string nraenv
-      := silent_optimizer_logger string nraenv.
-    Definition compiler_nnrc_optimizer_logger : optimizer_logger string nnrc
-      := silent_optimizer_logger string nnrc.
-    Definition compiler_nnrs_imp_expr_optimizer_logger : optimizer_logger string nnrs_imp_expr
-      := silent_optimizer_logger string nnrs_imp_expr.
-    Definition compiler_nnrs_imp_stmt_optimizer_logger : optimizer_logger string nnrs_imp_stmt
-      := silent_optimizer_logger string nnrs_imp_stmt.
-    Definition compiler_nnrs_imp_optimizer_logger : optimizer_logger string nnrs_imp
-      := silent_optimizer_logger string nnrs_imp.
-    Definition compiler_dnnrc_optimizer_logger {br:brand_relation}: optimizer_logger string (@dnnrc_base _ (type_annotation unit) dataframe)
-      := silent_optimizer_logger string (@dnnrc_base _ (type_annotation unit) dataframe).
-    Definition compiler_foreign_data_typing : foreign_data_typing
-      := trivial_foreign_data_typing.
-    
-  End TrivialRuntime.
+Module TrivialRuntime <: CompilerRuntime.
+  Definition compiler_foreign_type : foreign_type
+    := trivial_foreign_type.
+  Definition compiler_foreign_runtime : foreign_runtime
+    := trivial_foreign_runtime.
+  Definition compiler_foreign_to_java : foreign_to_java
+    := trivial_foreign_to_java.
+  Definition compiler_foreign_to_javascript : foreign_to_javascript
+    := trivial_foreign_to_javascript.
+  Definition compiler_foreign_to_ajavascript : foreign_to_ajavascript
+    := trivial_foreign_to_ajavascript.
+  Definition compiler_foreign_ejson_to_ajavascript : foreign_ejson_to_ajavascript
+    := trivial_foreign_ejson_to_ajavascript.
+  Definition compiler_foreign_to_scala : foreign_to_scala
+    := trivial_foreign_to_scala.
+  Definition compiler_foreign_to_ejson : foreign_to_ejson
+    := trivial_foreign_to_ejson.
+  Definition compiler_foreign_type_to_JSON : foreign_type_to_JSON
+    := trivial_foreign_type_to_JSON.
+  Definition compiler_foreign_reduce_op : foreign_reduce_op
+    := trivial_foreign_reduce_op.
+  Definition compiler_foreign_to_reduce_op : foreign_to_reduce_op
+    := trivial_foreign_to_reduce_op.
+  Definition compiler_foreign_to_spark : foreign_to_spark
+    := trivial_foreign_to_spark.
+  Definition compiler_nraenv_optimizer_logger : optimizer_logger string nraenv
+    := silent_optimizer_logger string nraenv.
+  Definition compiler_nnrc_optimizer_logger : optimizer_logger string nnrc
+    := silent_optimizer_logger string nnrc.
+  Definition compiler_nnrs_imp_expr_optimizer_logger : optimizer_logger string nnrs_imp_expr
+    := silent_optimizer_logger string nnrs_imp_expr.
+  Definition compiler_nnrs_imp_stmt_optimizer_logger : optimizer_logger string nnrs_imp_stmt
+    := silent_optimizer_logger string nnrs_imp_stmt.
+  Definition compiler_nnrs_imp_optimizer_logger : optimizer_logger string nnrs_imp
+    := silent_optimizer_logger string nnrs_imp.
+  Definition compiler_dnnrc_optimizer_logger {br:brand_relation}: optimizer_logger string (@dnnrc_base _ (type_annotation unit) dataframe)
+    := silent_optimizer_logger string (@dnnrc_base _ (type_annotation unit) dataframe).
+  Definition compiler_foreign_data_typing : foreign_data_typing
+    := trivial_foreign_data_typing.
+End TrivialRuntime.
 
-  Module TrivialForeignType <: CompilerForeignType.
-    Definition compiler_foreign_type : foreign_type
-      := trivial_foreign_type.
-  End TrivialForeignType.
+Module TrivialForeignType <: CompilerForeignType.
+  Definition compiler_foreign_type : foreign_type
+    := trivial_foreign_type.
+End TrivialForeignType.
   
-  Module TrivialModel(bm:CompilerBrandModel(TrivialForeignType)) <: CompilerModel.
-    Definition compiler_foreign_type : foreign_type
-      := trivial_foreign_type.
-    Definition compiler_basic_model : @basic_model
-      := @trivial_basic_model bm.compiler_brand_model.
-    Definition compiler_model_foreign_to_java : foreign_to_java
-      := trivial_foreign_to_java.
-    Definition compiler_model_foreign_to_javascript : foreign_to_javascript
-      := trivial_foreign_to_javascript.
-    Definition compiler_model_foreign_to_ajavascript : foreign_to_ajavascript
-      := trivial_foreign_to_ajavascript.
-    Definition compiler_model_foreign_to_scala : foreign_to_scala
-      := trivial_foreign_to_scala.
-    Definition compiler_model_foreign_to_JSON : foreign_to_JSON
-      := trivial_foreign_to_JSON.
-    Definition compiler_model_foreign_type_to_JSON : foreign_type_to_JSON
-      := trivial_foreign_type_to_JSON.
-    Definition compiler_model_foreign_reduce_op : foreign_reduce_op
-      := trivial_foreign_reduce_op.
-    Definition compiler_model_foreign_to_reduce_op : foreign_to_reduce_op
-      := trivial_foreign_to_reduce_op.
-    Definition compiler_model_foreign_to_spark : foreign_to_spark
-      := trivial_foreign_to_spark.
-    Definition compiler_model_nraenv_optimizer_logger : optimizer_logger string nraenv
-      := silent_optimizer_logger string nraenv.
-    Definition compiler_model_nnrc_optimizer_logger : optimizer_logger string nnrc
-      := silent_optimizer_logger string nnrc.
-    Definition compiler_model_nnrs_imp_expr_optimizer_logger : optimizer_logger string nnrs_imp_expr
-      := silent_optimizer_logger string nnrs_imp_expr.
-    Definition compiler_model_nnrs_imp_stmt_optimizer_logger : optimizer_logger string nnrs_imp_stmt
-      := silent_optimizer_logger string nnrs_imp_stmt.
-    Definition compiler_model_nnrs_imp_optimizer_logger : optimizer_logger string nnrs_imp
-      := silent_optimizer_logger string nnrs_imp.
-    Definition compiler_model_dnnrc_optimizer_logger {br:brand_relation}: optimizer_logger string (@dnnrc_base _ (type_annotation unit) dataframe)
-      := silent_optimizer_logger string (@dnnrc_base _ (type_annotation unit) dataframe).
-    Definition compiler_model_foreign_data_typing : foreign_data_typing
-      := trivial_foreign_data_typing.
-  End TrivialModel.
+Module TrivialModel(bm:CompilerBrandModel(TrivialForeignType)) <: CompilerModel.
+  Definition compiler_foreign_type : foreign_type
+    := trivial_foreign_type.
+  Definition compiler_basic_model : @basic_model
+    := @trivial_basic_model bm.compiler_brand_model.
+  Definition compiler_model_foreign_to_java : foreign_to_java
+    := trivial_foreign_to_java.
+  Definition compiler_model_foreign_to_javascript : foreign_to_javascript
+    := trivial_foreign_to_javascript.
+  Definition compiler_model_foreign_to_ajavascript : foreign_to_ajavascript
+    := trivial_foreign_to_ajavascript.
+  Definition compiler_model_foreign_ejson_to_ajavascript : foreign_ejson_to_ajavascript
+    := trivial_foreign_ejson_to_ajavascript.
+  Definition compiler_model_foreign_to_scala : foreign_to_scala
+    := trivial_foreign_to_scala.
+  Definition compiler_model_foreign_to_ejson : foreign_to_ejson
+    := trivial_foreign_to_ejson.
+  Definition compiler_model_foreign_type_to_JSON : foreign_type_to_JSON
+    := trivial_foreign_type_to_JSON.
+  Definition compiler_model_foreign_reduce_op : foreign_reduce_op
+    := trivial_foreign_reduce_op.
+  Definition compiler_model_foreign_to_reduce_op : foreign_to_reduce_op
+    := trivial_foreign_to_reduce_op.
+  Definition compiler_model_foreign_to_spark : foreign_to_spark
+    := trivial_foreign_to_spark.
+  Definition compiler_model_nraenv_optimizer_logger : optimizer_logger string nraenv
+    := silent_optimizer_logger string nraenv.
+  Definition compiler_model_nnrc_optimizer_logger : optimizer_logger string nnrc
+    := silent_optimizer_logger string nnrc.
+  Definition compiler_model_nnrs_imp_expr_optimizer_logger : optimizer_logger string nnrs_imp_expr
+    := silent_optimizer_logger string nnrs_imp_expr.
+  Definition compiler_model_nnrs_imp_stmt_optimizer_logger : optimizer_logger string nnrs_imp_stmt
+    := silent_optimizer_logger string nnrs_imp_stmt.
+  Definition compiler_model_nnrs_imp_optimizer_logger : optimizer_logger string nnrs_imp
+    := silent_optimizer_logger string nnrs_imp.
+  Definition compiler_model_dnnrc_optimizer_logger {br:brand_relation}: optimizer_logger string (@dnnrc_base _ (type_annotation unit) dataframe)
+    := silent_optimizer_logger string (@dnnrc_base _ (type_annotation unit) dataframe).
+  Definition compiler_model_foreign_data_typing : foreign_data_typing
+    := trivial_foreign_data_typing.
+End TrivialModel.
 
